rocq/theories/TypeSystem/TypeSafetyCallFrameShadowSafe.v
@@ -222,6 +222,14 @@ Proof.
   - eapply TERS_MakeClosure; eauto.
   - eapply TERS_MakeClosure_Static; eauto.
   - eapply TERS_CallExpr_MakeClosure; eauto.
+  - eapply TERS_CallExpr_Fn.
+    + exact n0.
+    + apply H. eapply root_env_tail_fresh_names_app_l. exact H1.
+    + apply H0. eapply root_env_tail_fresh_names_app_r. exact H1.
+  - eapply TERS_CallExpr_Closure.
+    + exact n0.
+    + apply H. eapply root_env_tail_fresh_names_app_l. exact H1.
+    + apply H0. eapply root_env_tail_fresh_names_app_r. exact H1.
   - eapply TERS_Struct; eauto.
   - eapply TERS_Enum; eauto.
   - pose proof (root_env_tail_fresh_names_app_l _ _ _ H2) as Hfresh_scrut.
